theories/lr_lemmasTSel.v
@@ -14,9 +14,9 @@ Section Sec.
   Proof.
     iIntros "/= #Hva !>" (v ρ) "#Hg #HvL !>".
     iDestruct ("Hva" $! ρ with "Hg") as (ds) "#[% #H]"; iClear "Hva".
-    iDestruct "H" as (φ) "#[Hl [HLφ HφU]]".
+    iDestruct "H" as (φ σ) "#[Hl [HLφ HφU]]".
     simplOpen ds'; simpl.
-    iExists (vobj ds'), φ, ds.
+    iExists (vobj ds'), σ, φ, ds.
     repeat iSplit; trivial.
     - iApply "HφU"; iApply "HLφ"; iApply "HvL".
     -
@@ -32,9 +32,9 @@ Section Sec.
   Proof.
     iIntros "/= #Hva !>" (v ρ) "#Hg #HvL !>".
     iDestruct ("Hva" $! ρ with "Hg") as (ds) "#[% #H]"; iClear "Hva".
-    iDestruct "H" as (φ) "#[Hl [HLφ HφU]]".
+    iDestruct "H" as (φ σ) "#[Hl [HLφ HφU]]".
     simplOpen ds'; simpl.
-    iExists (vobj ds'), φ, ds.
+    iExists (vobj ds'), σ , φ, ds.
     repeat iSplit; trivial.
     iRight; iApply "HLφ". iApply "HvL".
   Qed.
@@ -45,12 +45,12 @@ Section Sec.
   Proof.
     iIntros "/= #Hva !>" (v ρ) "#Hg #Hφ".
     iDestruct ("Hva" $! ρ with "Hg") as (ds) "#[% #H]"; iClear "Hva".
-    iDestruct "H" as (φ) "#[Hlφ [HLφ HφU]]".
+    iDestruct "H" as (φ σ) "#[Hlφ [HLφ HφU]]".
     iDestruct "Hlφ" as (γ) "[% Hγφ]".
 
     iApply "HφU".
     simplOpen ds'; simpl.
-    iDestruct "Hφ" as (va1 φ1 ds1) "[% [% [Hlφ1 [_ [[] | Hφ1v]]]]] /=".
+    iDestruct "Hφ" as (va1 σ1 φ1 ds1) "[% [% [Hlφ1 [_ [[] | Hφ1v]]]]] /=".
     iDestruct "Hlφ1" as (γ1) "[% Hγφ1]".
 
     injectHyps; openDet; optFuncs_det.
